$$
\begin{aligned} 
P_{1}\ &=\left(0,0\right)+\left(v_{0}\cdot\cos\left(b\right),v_{0}\cdot\sin\left(b\right)\right)\left(t_{ime}-t_{factor}\right)\ t+\ \left(0,-\frac{1}{2}g\left(t_{ime}-t_{factor}\right)^{2}\right)t^{2}\ \left\{t_{ime}-t_{factor}>0\right\}\\

P_{2}&=\left(0,0\right)+\left(-v_{0}\cdot\cos\left(b\right),v_{0}\cdot\sin\left(b\right)\right)\left(t_{ime}-t_{factor}\right)\ t+\ \left(0,-\frac{1}{2}g\left(t_{ime}-t_{factor}\right)^{2}\right)t^{2}\ \left\{t_{ime}-t_{factor}>0\right\}\\

b&=\left(\left[0,\frac{\pi}{12},...,\frac{\pi}{2}\right]-\frac{\pi}{24}\right)\left[1,...7\right]\\

v_{0}\ &=\left(\left[0,5,...,30\right]+5\right)\\

t_{factor}&=\left[0,1,...,6\right]
\end{aligned}
$$
